$$(f+g) \left([tx^p + (1-t)y^p]^{\frac{1}{p}}\right) = \left[f \left([tx^p + (1-t)y^p]^{\frac{1}{p}}\right)\right] + \left[g \left([tx^p + (1-t)y^p]^{\frac{1}{p}}\right)\right] \le \left[ \frac{1}{n} \sum_{i=1}^{n} t^{\frac{1}{i}} f(x) + \frac{1}{n} \sum_{i=1}^{n} (1-t)^{\frac{1}{i}} f(y) \right] + \left[ \frac{1}{n} \sum_{i=1}^{n} t^{\frac{1}{i}} g(x) + \frac{1}{n} \sum_{i=1}^{n} (1-t)^{\frac{1}{i}} g(y) \right] = \frac{1}{n} \sum_{i=1}^{n} t^{\frac{1}{i}} (f+g)(x) + \frac{1}{n} \sum_{i=1}^{n} (1-t)^{\frac{1}{i}} (f+g)(y)$$